tests/coq/array/Array_Funs.v
@@ -10,16 +10,21 @@ Require Export Array_Types.
 Import Array_Types.
 Module Array_Funs.
 
+(** [array::incr]: merged forward/backward function
+    (there is a single backward function, and the forward function returns ()) *)
+Definition incr (x : u32) : result u32 :=
+  u32_add x 1%u32.
+
 (** [array::array_to_shared_slice_]: forward function *)
-Definition array_to_shared_slice__fwd
+Definition array_to_shared_slice_
   (T : Type) (s : array T 32%usize) : result (slice T) :=
-  array_to_slice_shared T 32%usize s
+  array_to_slice T 32%usize s
 .
 
 (** [array::array_to_mut_slice_]: forward function *)
-Definition array_to_mut_slice__fwd
+Definition array_to_mut_slice_
   (T : Type) (s : array T 32%usize) : result (slice T) :=
-  array_to_slice_mut_fwd T 32%usize s
+  array_to_slice T 32%usize s
 .
 
 (** [array::array_to_mut_slice_]: backward function 0 *)
@@ -27,58 +32,44 @@ Definition array_to_mut_slice__back
   (T : Type) (s : array T 32%usize) (ret : slice T) :
   result (array T 32%usize)
   :=
-  array_to_slice_mut_back T 32%usize s ret
+  array_from_slice T 32%usize s ret
 .
 
 (** [array::array_len]: forward function *)
-Definition array_len_fwd (T : Type) (s : array T 32%usize) : result usize :=
-  s0 <- array_to_slice_shared T 32%usize s; let i := slice_len T s0 in Return i
+Definition array_len (T : Type) (s : array T 32%usize) : result usize :=
+  s0 <- array_to_slice T 32%usize s; let i := slice_len T s0 in Return i
 .
 
 (** [array::shared_array_len]: forward function *)
-Definition shared_array_len_fwd
-  (T : Type) (s : array T 32%usize) : result usize :=
-  s0 <- array_to_slice_shared T 32%usize s; let i := slice_len T s0 in Return i
+Definition shared_array_len (T : Type) (s : array T 32%usize) : result usize :=
+  s0 <- array_to_slice T 32%usize s; let i := slice_len T s0 in Return i
 .
 
 (** [array::shared_slice_len]: forward function *)
-Definition shared_slice_len_fwd (T : Type) (s : slice T) : result usize :=
+Definition shared_slice_len (T : Type) (s : slice T) : result usize :=
   let i := slice_len T s in Return i
 .
 
 (** [array::index_array_shared]: forward function *)
-Definition index_array_shared_fwd
+Definition index_array_shared
   (T : Type) (s : array T 32%usize) (i : usize) : result T :=
-  array_index_shared T 32%usize s i
+  array_index_usize T 32%usize s i
 .
 
 (** [array::index_array_u32]: forward function *)
-Definition index_array_u32_fwd
-  (s : array u32 32%usize) (i : usize) : result u32 :=
-  array_index_shared u32 32%usize s i
-.
-
-(** [array::index_array_generic]: forward function *)
-Definition index_array_generic_fwd
-  (N : usize) (s : array u32 N) (i : usize) : result u32 :=
-  array_index_shared u32 N s i
-.
-
-(** [array::index_array_generic_call]: forward function *)
-Definition index_array_generic_call_fwd
-  (N : usize) (s : array u32 N) (i : usize) : result u32 :=
-  index_array_generic_fwd N s i
+Definition index_array_u32 (s : array u32 32%usize) (i : usize) : result u32 :=
+  array_index_usize u32 32%usize s i
 .
 
 (** [array::index_array_copy]: forward function *)
-Definition index_array_copy_fwd (x : array u32 32%usize) : result u32 :=
-  array_index_shared u32 32%usize x 0%usize
+Definition index_array_copy (x : array u32 32%usize) : result u32 :=
+  array_index_usize u32 32%usize x 0%usize
 .
 
 (** [array::index_mut_array]: forward function *)
-Definition index_mut_array_fwd
+Definition index_mut_array
   (T : Type) (s : array T 32%usize) (i : usize) : result T :=
-  array_index_mut_fwd T 32%usize s i
+  array_index_usize T 32%usize s i
 .
 
 (** [array::index_mut_array]: backward function 0 *)
@@ -86,298 +77,314 @@ Definition index_mut_array_back
   (T : Type) (s : array T 32%usize) (i : usize) (ret : T) :
   result (array T 32%usize)
   :=
-  array_index_mut_back T 32%usize s i ret
+  array_update_usize T 32%usize s i ret
 .
 
 (** [array::index_slice]: forward function *)
-Definition index_slice_fwd (T : Type) (s : slice T) (i : usize) : result T :=
-  slice_index_shared T s i
+Definition index_slice (T : Type) (s : slice T) (i : usize) : result T :=
+  slice_index_usize T s i
 .
 
 (** [array::index_mut_slice]: forward function *)
-Definition index_mut_slice_fwd
-  (T : Type) (s : slice T) (i : usize) : result T :=
-  slice_index_mut_fwd T s i
+Definition index_mut_slice (T : Type) (s : slice T) (i : usize) : result T :=
+  slice_index_usize T s i
 .
 
 (** [array::index_mut_slice]: backward function 0 *)
 Definition index_mut_slice_back
   (T : Type) (s : slice T) (i : usize) (ret : T) : result (slice T) :=
-  slice_index_mut_back T s i ret
+  slice_update_usize T s i ret
 .
 
 (** [array::slice_subslice_shared_]: forward function *)
-Definition slice_subslice_shared__fwd
-  (x : slice u32) (y : usize) (z : usize) : result (slice u32) :=
-  slice_subslice_shared u32 x (mk_range y z)
+Definition slice_subslice_shared_
+  (n : nat) (x : slice u32) (y : usize) (z : usize) : result (slice u32) :=
+  core_slice_index_Slice_index u32 (core_ops_range_Range usize)
+    (core_slice_index_Range_coresliceindexSliceIndexInst u32) x
+    {| core_ops_range_Range_start := y; core_ops_range_Range_end_ := z |}
 .
 
 (** [array::slice_subslice_mut_]: forward function *)
-Definition slice_subslice_mut__fwd
-  (x : slice u32) (y : usize) (z : usize) : result (slice u32) :=
-  slice_subslice_mut_fwd u32 x (mk_range y z)
+Definition slice_subslice_mut_
+  (n : nat) (x : slice u32) (y : usize) (z : usize) : result (slice u32) :=
+  core_slice_index_Slice_index_mut u32 (core_ops_range_Range usize)
+    (core_slice_index_Range_coresliceindexSliceIndexInst u32) x
+    {| core_ops_range_Range_start := y; core_ops_range_Range_end_ := z |}
 .
 
 (** [array::slice_subslice_mut_]: backward function 0 *)
 Definition slice_subslice_mut__back
-  (x : slice u32) (y : usize) (z : usize) (ret : slice u32) :
+  (n : nat) (x : slice u32) (y : usize) (z : usize) (ret : slice u32) :
   result (slice u32)
   :=
-  slice_subslice_mut_back u32 x (mk_range y z) ret
+  core_slice_index_Slice_index_mut_back u32 (core_ops_range_Range usize)
+    (core_slice_index_Range_coresliceindexSliceIndexInst u32) x
+    {| core_ops_range_Range_start := y; core_ops_range_Range_end_ := z |} ret
 .
 
 (** [array::array_to_slice_shared_]: forward function *)
-Definition array_to_slice_shared__fwd
+Definition array_to_slice_shared_
   (x : array u32 32%usize) : result (slice u32) :=
-  array_to_slice_shared u32 32%usize x
+  array_to_slice u32 32%usize x
 .
 
 (** [array::array_to_slice_mut_]: forward function *)
-Definition array_to_slice_mut__fwd
-  (x : array u32 32%usize) : result (slice u32) :=
-  array_to_slice_mut_fwd u32 32%usize x
+Definition array_to_slice_mut_ (x : array u32 32%usize) : result (slice u32) :=
+  array_to_slice u32 32%usize x
 .
 
 (** [array::array_to_slice_mut_]: backward function 0 *)
 Definition array_to_slice_mut__back
   (x : array u32 32%usize) (ret : slice u32) : result (array u32 32%usize) :=
-  array_to_slice_mut_back u32 32%usize x ret
+  array_from_slice u32 32%usize x ret
 .
 
 (** [array::array_subslice_shared_]: forward function *)
-Definition array_subslice_shared__fwd
-  (x : array u32 32%usize) (y : usize) (z : usize) : result (slice u32) :=
-  array_subslice_shared u32 32%usize x (mk_range y z)
+Definition array_subslice_shared_
+  (n : nat) (x : array u32 32%usize) (y : usize) (z : usize) :
+  result (slice u32)
+  :=
+  core_array_Array_index u32 (core_ops_range_Range usize) 32%usize
+    (core_slice_index_Slice_coreopsindexIndexInst u32 (core_ops_range_Range
+    usize) (core_slice_index_Range_coresliceindexSliceIndexInst u32)) x
+    {| core_ops_range_Range_start := y; core_ops_range_Range_end_ := z |}
 .
 
 (** [array::array_subslice_mut_]: forward function *)
-Definition array_subslice_mut__fwd
-  (x : array u32 32%usize) (y : usize) (z : usize) : result (slice u32) :=
-  array_subslice_mut_fwd u32 32%usize x (mk_range y z)
+Definition array_subslice_mut_
+  (n : nat) (x : array u32 32%usize) (y : usize) (z : usize) :
+  result (slice u32)
+  :=
+  core_array_Array_index_mut u32 (core_ops_range_Range usize) 32%usize
+    (core_slice_index_Slice_coreopsindexIndexMutInst u32 (core_ops_range_Range
+    usize) (core_slice_index_Range_coresliceindexSliceIndexInst u32)) x
+    {| core_ops_range_Range_start := y; core_ops_range_Range_end_ := z |}
 .
 
 (** [array::array_subslice_mut_]: backward function 0 *)
 Definition array_subslice_mut__back
-  (x : array u32 32%usize) (y : usize) (z : usize) (ret : slice u32) :
+  (n : nat) (x : array u32 32%usize) (y : usize) (z : usize) (ret : slice u32)
+  :
   result (array u32 32%usize)
   :=
-  array_subslice_mut_back u32 32%usize x (mk_range y z) ret
+  core_array_Array_index_mut_back u32 (core_ops_range_Range usize) 32%usize
+    (core_slice_index_Slice_coreopsindexIndexMutInst u32 (core_ops_range_Range
+    usize) (core_slice_index_Range_coresliceindexSliceIndexInst u32)) x
+    {| core_ops_range_Range_start := y; core_ops_range_Range_end_ := z |} ret
 .
 
 (** [array::index_slice_0]: forward function *)
-Definition index_slice_0_fwd (T : Type) (s : slice T) : result T :=
-  slice_index_shared T s 0%usize
+Definition index_slice_0 (T : Type) (s : slice T) : result T :=
+  slice_index_usize T s 0%usize
 .
 
 (** [array::index_array_0]: forward function *)
-Definition index_array_0_fwd (T : Type) (s : array T 32%usize) : result T :=
-  array_index_shared T 32%usize s 0%usize
+Definition index_array_0 (T : Type) (s : array T 32%usize) : result T :=
+  array_index_usize T 32%usize s 0%usize
 .
 
 (** [array::index_index_array]: forward function *)
-Definition index_index_array_fwd
+Definition index_index_array
   (s : array (array u32 32%usize) 32%usize) (i : usize) (j : usize) :
   result u32
   :=
-  a <- array_index_shared (array u32 32%usize) 32%usize s i;
-  array_index_shared u32 32%usize a j
+  a <- array_index_usize (array u32 32%usize) 32%usize s i;
+  array_index_usize u32 32%usize a j
 .
 
-(** [array::const_gen_ret]: forward function *)
-Definition const_gen_ret_fwd (N : usize) : result usize :=
-  Return N.
-
 (** [array::update_update_array]: forward function *)
-Definition update_update_array_fwd
+Definition update_update_array
   (s : array (array u32 32%usize) 32%usize) (i : usize) (j : usize) :
   result unit
   :=
-  a <- array_index_mut_fwd (array u32 32%usize) 32%usize s i;
-  a0 <- array_index_mut_back u32 32%usize a j 0%u32;
-  _ <- array_index_mut_back (array u32 32%usize) 32%usize s i a0;
+  a <- array_index_usize (array u32 32%usize) 32%usize s i;
+  a0 <- array_update_usize u32 32%usize a j 0%u32;
+  _ <- array_update_usize (array u32 32%usize) 32%usize s i a0;
   Return tt
 .
 
 (** [array::array_local_deep_copy]: forward function *)
-Definition array_local_deep_copy_fwd (x : array u32 32%usize) : result unit :=
+Definition array_local_deep_copy (x : array u32 32%usize) : result unit :=
   Return tt
 .
 
 (** [array::take_array]: forward function *)
-Definition take_array_fwd (a : array u32 2%usize) : result unit :=
+Definition take_array (a : array u32 2%usize) : result unit :=
   Return tt.
 
 (** [array::take_array_borrow]: forward function *)
-Definition take_array_borrow_fwd (a : array u32 2%usize) : result unit :=
+Definition take_array_borrow (a : array u32 2%usize) : result unit :=
   Return tt
 .
 
 (** [array::take_slice]: forward function *)
-Definition take_slice_fwd (s : slice u32) : result unit :=
+Definition take_slice (s : slice u32) : result unit :=
   Return tt.
 
 (** [array::take_mut_slice]: merged forward/backward function
     (there is a single backward function, and the forward function returns ()) *)
-Definition take_mut_slice_fwd_back (s : slice u32) : result (slice u32) :=
-  Return s
-.
+Definition take_mut_slice (s : slice u32) : result (slice u32) :=
+  Return s.
 
 (** [array::take_all]: forward function *)
-Definition take_all_fwd : result unit :=
-  _ <- take_array_fwd (mk_array u32 2%usize [ 0%u32; 0%u32 ]);
-  _ <- take_array_borrow_fwd (mk_array u32 2%usize [ 0%u32; 0%u32 ]);
-  s <-
-    array_to_slice_shared u32 2%usize (mk_array u32 2%usize [ 0%u32; 0%u32 ]);
-  _ <- take_slice_fwd s;
-  s0 <-
-    array_to_slice_mut_fwd u32 2%usize (mk_array u32 2%usize [ 0%u32; 0%u32 ]);
-  s1 <- take_mut_slice_fwd_back s0;
-  _ <-
-    array_to_slice_mut_back u32 2%usize (mk_array u32 2%usize [ 0%u32; 0%u32 ])
-      s1;
+Definition take_all : result unit :=
+  _ <- take_array (mk_array u32 2%usize [ 0%u32; 0%u32 ]);
+  _ <- take_array_borrow (mk_array u32 2%usize [ 0%u32; 0%u32 ]);
+  s <- array_to_slice u32 2%usize (mk_array u32 2%usize [ 0%u32; 0%u32 ]);
+  _ <- take_slice s;
+  s0 <- array_to_slice u32 2%usize (mk_array u32 2%usize [ 0%u32; 0%u32 ]);
+  s1 <- take_mut_slice s0;
+  _ <- array_from_slice u32 2%usize (mk_array u32 2%usize [ 0%u32; 0%u32 ]) s1;
   Return tt
 .
 
 (** [array::index_array]: forward function *)
-Definition index_array_fwd (x : array u32 2%usize) : result u32 :=
-  array_index_shared u32 2%usize x 0%usize
+Definition index_array (x : array u32 2%usize) : result u32 :=
+  array_index_usize u32 2%usize x 0%usize
 .
 
 (** [array::index_array_borrow]: forward function *)
-Definition index_array_borrow_fwd (x : array u32 2%usize) : result u32 :=
-  array_index_shared u32 2%usize x 0%usize
+Definition index_array_borrow (x : array u32 2%usize) : result u32 :=
+  array_index_usize u32 2%usize x 0%usize
 .
 
 (** [array::index_slice_u32_0]: forward function *)
-Definition index_slice_u32_0_fwd (x : slice u32) : result u32 :=
-  slice_index_shared u32 x 0%usize
+Definition index_slice_u32_0 (x : slice u32) : result u32 :=
+  slice_index_usize u32 x 0%usize
 .
 
 (** [array::index_mut_slice_u32_0]: forward function *)
-Definition index_mut_slice_u32_0_fwd (x : slice u32) : result u32 :=
-  slice_index_shared u32 x 0%usize
+Definition index_mut_slice_u32_0 (x : slice u32) : result u32 :=
+  slice_index_usize u32 x 0%usize
 .
 
 (** [array::index_mut_slice_u32_0]: backward function 0 *)
 Definition index_mut_slice_u32_0_back (x : slice u32) : result (slice u32) :=
-  _ <- slice_index_shared u32 x 0%usize; Return x
+  _ <- slice_index_usize u32 x 0%usize; Return x
 .
 
 (** [array::index_all]: forward function *)
-Definition index_all_fwd : result u32 :=
-  i <- index_array_fwd (mk_array u32 2%usize [ 0%u32; 0%u32 ]);
-  i0 <- index_array_fwd (mk_array u32 2%usize [ 0%u32; 0%u32 ]);
+Definition index_all : result u32 :=
+  i <- index_array (mk_array u32 2%usize [ 0%u32; 0%u32 ]);
+  i0 <- index_array (mk_array u32 2%usize [ 0%u32; 0%u32 ]);
   i1 <- u32_add i i0;
-  i2 <- index_array_borrow_fwd (mk_array u32 2%usize [ 0%u32; 0%u32 ]);
+  i2 <- index_array_borrow (mk_array u32 2%usize [ 0%u32; 0%u32 ]);
   i3 <- u32_add i1 i2;
-  s <-
-    array_to_slice_shared u32 2%usize (mk_array u32 2%usize [ 0%u32; 0%u32 ]);
-  i4 <- index_slice_u32_0_fwd s;
+  s <- array_to_slice u32 2%usize (mk_array u32 2%usize [ 0%u32; 0%u32 ]);
+  i4 <- index_slice_u32_0 s;
   i5 <- u32_add i3 i4;
-  s0 <-
-    array_to_slice_mut_fwd u32 2%usize (mk_array u32 2%usize [ 0%u32; 0%u32 ]);
-  i6 <- index_mut_slice_u32_0_fwd s0;
+  s0 <- array_to_slice u32 2%usize (mk_array u32 2%usize [ 0%u32; 0%u32 ]);
+  i6 <- index_mut_slice_u32_0 s0;
   i7 <- u32_add i5 i6;
   s1 <- index_mut_slice_u32_0_back s0;
-  _ <-
-    array_to_slice_mut_back u32 2%usize (mk_array u32 2%usize [ 0%u32; 0%u32 ])
-      s1;
+  _ <- array_from_slice u32 2%usize (mk_array u32 2%usize [ 0%u32; 0%u32 ]) s1;
   Return i7
 .
 
 (** [array::update_array]: forward function *)
-Definition update_array_fwd (x : array u32 2%usize) : result unit :=
-  _ <- array_index_mut_back u32 2%usize x 0%usize 1%u32; Return tt
+Definition update_array (x : array u32 2%usize) : result unit :=
+  _ <- array_update_usize u32 2%usize x 0%usize 1%u32; Return tt
 .
 
 (** [array::update_array_mut_borrow]: merged forward/backward function
     (there is a single backward function, and the forward function returns ()) *)
-Definition update_array_mut_borrow_fwd_back
+Definition update_array_mut_borrow
   (x : array u32 2%usize) : result (array u32 2%usize) :=
-  array_index_mut_back u32 2%usize x 0%usize 1%u32
+  array_update_usize u32 2%usize x 0%usize 1%u32
 .
 
 (** [array::update_mut_slice]: merged forward/backward function
     (there is a single backward function, and the forward function returns ()) *)
-Definition update_mut_slice_fwd_back (x : slice u32) : result (slice u32) :=
-  slice_index_mut_back u32 x 0%usize 1%u32
+Definition update_mut_slice (x : slice u32) : result (slice u32) :=
+  slice_update_usize u32 x 0%usize 1%u32
 .
 
 (** [array::update_all]: forward function *)
-Definition update_all_fwd : result unit :=
-  _ <- update_array_fwd (mk_array u32 2%usize [ 0%u32; 0%u32 ]);
-  x <-
-    update_array_mut_borrow_fwd_back (mk_array u32 2%usize [ 0%u32; 0%u32 ]);
-  s <- array_to_slice_mut_fwd u32 2%usize x;
-  s0 <- update_mut_slice_fwd_back s;
-  _ <- array_to_slice_mut_back u32 2%usize x s0;
+Definition update_all : result unit :=
+  _ <- update_array (mk_array u32 2%usize [ 0%u32; 0%u32 ]);
+  x <- update_array_mut_borrow (mk_array u32 2%usize [ 0%u32; 0%u32 ]);
+  s <- array_to_slice u32 2%usize x;
+  s0 <- update_mut_slice s;
+  _ <- array_from_slice u32 2%usize x s0;
   Return tt
 .
 
 (** [array::range_all]: forward function *)
-Definition range_all_fwd : result unit :=
+Definition range_all (n : nat) : result unit :=
   s <-
-    array_subslice_mut_fwd u32 4%usize
-      (mk_array u32 4%usize [ 0%u32; 0%u32; 0%u32; 0%u32 ]) (mk_range 1%usize
-      3%usize);
-  s0 <- update_mut_slice_fwd_back s;
+    core_array_Array_index_mut u32 (core_ops_range_Range usize) 4%usize
+      (core_slice_index_Slice_coreopsindexIndexMutInst u32
+      (core_ops_range_Range usize)
+      (core_slice_index_Range_coresliceindexSliceIndexInst u32))
+      (mk_array u32 4%usize [ 0%u32; 0%u32; 0%u32; 0%u32 ])
+      {|
+        core_ops_range_Range_start := 1%usize;
+        core_ops_range_Range_end_ := 3%usize
+      |};
+  s0 <- update_mut_slice s;
   _ <-
-    array_subslice_mut_back u32 4%usize
-      (mk_array u32 4%usize [ 0%u32; 0%u32; 0%u32; 0%u32 ]) (mk_range 1%usize
-      3%usize) s0;
+    core_array_Array_index_mut_back u32 (core_ops_range_Range usize) 4%usize
+      (core_slice_index_Slice_coreopsindexIndexMutInst u32
+      (core_ops_range_Range usize)
+      (core_slice_index_Range_coresliceindexSliceIndexInst u32))
+      (mk_array u32 4%usize [ 0%u32; 0%u32; 0%u32; 0%u32 ])
+      {|
+        core_ops_range_Range_start := 1%usize;
+        core_ops_range_Range_end_ := 3%usize
+      |} s0;
   Return tt
 .
 
 (** [array::deref_array_borrow]: forward function *)
-Definition deref_array_borrow_fwd (x : array u32 2%usize) : result u32 :=
-  array_index_shared u32 2%usize x 0%usize
+Definition deref_array_borrow (x : array u32 2%usize) : result u32 :=
+  array_index_usize u32 2%usize x 0%usize
 .
 
 (** [array::deref_array_mut_borrow]: forward function *)
-Definition deref_array_mut_borrow_fwd (x : array u32 2%usize) : result u32 :=
-  array_index_shared u32 2%usize x 0%usize
+Definition deref_array_mut_borrow (x : array u32 2%usize) : result u32 :=
+  array_index_usize u32 2%usize x 0%usize
 .
 
 (** [array::deref_array_mut_borrow]: backward function 0 *)
 Definition deref_array_mut_borrow_back
   (x : array u32 2%usize) : result (array u32 2%usize) :=
-  _ <- array_index_shared u32 2%usize x 0%usize; Return x
+  _ <- array_index_usize u32 2%usize x 0%usize; Return x
 .
 
 (** [array::take_array_t]: forward function *)
-Definition take_array_t_fwd (a : array T_t 2%usize) : result unit :=
+Definition take_array_t (a : array AB_t 2%usize) : result unit :=
   Return tt.
 
 (** [array::non_copyable_array]: forward function *)
-Definition non_copyable_array_fwd : result unit :=
-  _ <- take_array_t_fwd (mk_array T_t 2%usize [ TA; TB ]); Return tt
+Definition non_copyable_array : result unit :=
+  _ <- take_array_t (mk_array AB_t 2%usize [ AB_A; AB_B ]); Return tt
 .
 
 (** [array::sum]: loop 0: forward function *)
-Fixpoint sum_loop_fwd
-  (n : nat) (s : slice u32) (sum : u32) (i : usize) : result u32 :=
+Fixpoint sum_loop
+  (n : nat) (s : slice u32) (sum0 : u32) (i : usize) : result u32 :=
   match n with
   | O => Fail_ OutOfFuel
   | S n0 =>
     let i0 := slice_len u32 s in
     if i s< i0
     then (
-      i1 <- slice_index_shared u32 s i;
-      sum0 <- u32_add sum i1;
+      i1 <- slice_index_usize u32 s i;
+      sum1 <- u32_add sum0 i1;
       i2 <- usize_add i 1%usize;
-      sum_loop_fwd n0 s sum0 i2)
-    else Return sum
+      sum_loop n0 s sum1 i2)
+    else Return sum0
   end
 .
 
 (** [array::sum]: forward function *)
-Definition sum_fwd (n : nat) (s : slice u32) : result u32 :=
-  sum_loop_fwd n s 0%u32 0%usize
+Definition sum (n : nat) (s : slice u32) : result u32 :=
+  sum_loop n s 0%u32 0%usize
 .
 
 (** [array::sum2]: loop 0: forward function *)
-Fixpoint sum2_loop_fwd
-  (n : nat) (s : slice u32) (s2 : slice u32) (sum : u32) (i : usize) :
+Fixpoint sum2_loop
+  (n : nat) (s : slice u32) (s2 : slice u32) (sum0 : u32) (i : usize) :
   result u32
   :=
   match n with
@@ -386,69 +393,64 @@ Fixpoint sum2_loop_fwd
     let i0 := slice_len u32 s in
     if i s< i0
     then (
-      i1 <- slice_index_shared u32 s i;
-      i2 <- slice_index_shared u32 s2 i;
+      i1 <- slice_index_usize u32 s i;
+      i2 <- slice_index_usize u32 s2 i;
       i3 <- u32_add i1 i2;
-      sum0 <- u32_add sum i3;
+      sum1 <- u32_add sum0 i3;
       i4 <- usize_add i 1%usize;
-      sum2_loop_fwd n0 s s2 sum0 i4)
-    else Return sum
+      sum2_loop n0 s s2 sum1 i4)
+    else Return sum0
   end
 .
 
 (** [array::sum2]: forward function *)
-Definition sum2_fwd (n : nat) (s : slice u32) (s2 : slice u32) : result u32 :=
+Definition sum2 (n : nat) (s : slice u32) (s2 : slice u32) : result u32 :=
   let i := slice_len u32 s in
   let i0 := slice_len u32 s2 in
-  if negb (i s= i0) then Fail_ Failure else sum2_loop_fwd n s s2 0%u32 0%usize
+  if negb (i s= i0) then Fail_ Failure else sum2_loop n s s2 0%u32 0%usize
 .
 
 (** [array::f0]: forward function *)
-Definition f0_fwd : result unit :=
-  s <-
-    array_to_slice_mut_fwd u32 2%usize (mk_array u32 2%usize [ 1%u32; 2%u32 ]);
-  s0 <- slice_index_mut_back u32 s 0%usize 1%u32;
-  _ <-
-    array_to_slice_mut_back u32 2%usize (mk_array u32 2%usize [ 1%u32; 2%u32 ])
-      s0;
+Definition f0 : result unit :=
+  s <- array_to_slice u32 2%usize (mk_array u32 2%usize [ 1%u32; 2%u32 ]);
+  s0 <- slice_update_usize u32 s 0%usize 1%u32;
+  _ <- array_from_slice u32 2%usize (mk_array u32 2%usize [ 1%u32; 2%u32 ]) s0;
   Return tt
 .
 
 (** [array::f1]: forward function *)
-Definition f1_fwd : result unit :=
+Definition f1 : result unit :=
   _ <-
-    array_index_mut_back u32 2%usize (mk_array u32 2%usize [ 1%u32; 2%u32 ])
+    array_update_usize u32 2%usize (mk_array u32 2%usize [ 1%u32; 2%u32 ])
       0%usize 1%u32;
   Return tt
 .
 
 (** [array::f2]: forward function *)
-Definition f2_fwd (i : u32) : result unit :=
+Definition f2 (i : u32) : result unit :=
   Return tt.
 
 (** [array::f4]: forward function *)
-Definition f4_fwd
-  (x : array u32 32%usize) (y : usize) (z : usize) : result (slice u32) :=
-  array_subslice_shared u32 32%usize x (mk_range y z)
+Definition f4
+  (n : nat) (x : array u32 32%usize) (y : usize) (z : usize) :
+  result (slice u32)
+  :=
+  core_array_Array_index u32 (core_ops_range_Range usize) 32%usize
+    (core_slice_index_Slice_coreopsindexIndexInst u32 (core_ops_range_Range
+    usize) (core_slice_index_Range_coresliceindexSliceIndexInst u32)) x
+    {| core_ops_range_Range_start := y; core_ops_range_Range_end_ := z |}
 .
 
 (** [array::f3]: forward function *)
-Definition f3_fwd (n : nat) : result u32 :=
+Definition f3 (n : nat) : result u32 :=
   i <-
-    array_index_shared u32 2%usize (mk_array u32 2%usize [ 1%u32; 2%u32 ])
+    array_index_usize u32 2%usize (mk_array u32 2%usize [ 1%u32; 2%u32 ])
       0%usize;
-  _ <- f2_fwd i;
-  s <-
-    array_to_slice_shared u32 2%usize (mk_array u32 2%usize [ 1%u32; 2%u32 ]);
-  s0 <-
-    f4_fwd
-      (mk_array u32 32%usize [
-        0%u32; 0%u32; 0%u32; 0%u32; 0%u32; 0%u32; 0%u32; 0%u32; 0%u32; 0%u32;
-        0%u32; 0%u32; 0%u32; 0%u32; 0%u32; 0%u32; 0%u32; 0%u32; 0%u32; 0%u32;
-        0%u32; 0%u32; 0%u32; 0%u32; 0%u32; 0%u32; 0%u32; 0%u32; 0%u32; 0%u32;
-        0%u32; 0%u32
-        ]) 16%usize 18%usize;
-  sum2_fwd n s s0
+  _ <- f2 i;
+  let b := array_repeat u32 32%usize 0%u32 in
+  s <- array_to_slice u32 2%usize (mk_array u32 2%usize [ 1%u32; 2%u32 ]);
+  s0 <- f4 n b 16%usize 18%usize;
+  sum2 n s s0
 .
 
 (** [array::SZ] *)
@@ -456,24 +458,18 @@ Definition sz_body : result usize := Return 32%usize.
 Definition sz_c : usize := sz_body%global.
 
 (** [array::f5]: forward function *)
-Definition f5_fwd (x : array u32 32%usize) : result u32 :=
-  array_index_shared u32 32%usize x 0%usize
+Definition f5 (x : array u32 32%usize) : result u32 :=
+  array_index_usize u32 32%usize x 0%usize
 .
 
 (** [array::ite]: forward function *)
-Definition ite_fwd : result unit :=
-  s <-
-    array_to_slice_mut_fwd u32 2%usize (mk_array u32 2%usize [ 0%u32; 0%u32 ]);
-  s0 <-
-    array_to_slice_mut_fwd u32 2%usize (mk_array u32 2%usize [ 0%u32; 0%u32 ]);
+Definition ite : result unit :=
+  s <- array_to_slice u32 2%usize (mk_array u32 2%usize [ 0%u32; 0%u32 ]);
+  s0 <- array_to_slice u32 2%usize (mk_array u32 2%usize [ 0%u32; 0%u32 ]);
   s1 <- index_mut_slice_u32_0_back s0;
-  _ <-
-    array_to_slice_mut_back u32 2%usize (mk_array u32 2%usize [ 0%u32; 0%u32 ])
-      s1;
+  _ <- array_from_slice u32 2%usize (mk_array u32 2%usize [ 0%u32; 0%u32 ]) s1;
   s2 <- index_mut_slice_u32_0_back s;
-  _ <-
-    array_to_slice_mut_back u32 2%usize (mk_array u32 2%usize [ 0%u32; 0%u32 ])
-      s2;
+  _ <- array_from_slice u32 2%usize (mk_array u32 2%usize [ 0%u32; 0%u32 ]) s2;
   Return tt
 .
 
