tests/coq/betree/BetreeMain_Opaque.v
@@ -11,29 +11,29 @@ Import BetreeMain_Types.
 Module BetreeMain_Opaque.
 
 (** [betree_main::betree_utils::load_internal_node]: forward function *)
-Axiom betree_utils_load_internal_node_fwd
-  : u64 -> state -> result (state * (Betree_list_t (u64 * Betree_message_t)))
+Axiom betree_utils_load_internal_node
+  : u64 -> state -> result (state * (betree_List_t (u64 * betree_Message_t)))
 .
 
 (** [betree_main::betree_utils::store_internal_node]: forward function *)
-Axiom betree_utils_store_internal_node_fwd
+Axiom betree_utils_store_internal_node
   :
-  u64 -> Betree_list_t (u64 * Betree_message_t) -> state -> result (state *
+  u64 -> betree_List_t (u64 * betree_Message_t) -> state -> result (state *
     unit)
 .
 
 (** [betree_main::betree_utils::load_leaf_node]: forward function *)
-Axiom betree_utils_load_leaf_node_fwd
-  : u64 -> state -> result (state * (Betree_list_t (u64 * u64)))
+Axiom betree_utils_load_leaf_node
+  : u64 -> state -> result (state * (betree_List_t (u64 * u64)))
 .
 
 (** [betree_main::betree_utils::store_leaf_node]: forward function *)
-Axiom betree_utils_store_leaf_node_fwd
-  : u64 -> Betree_list_t (u64 * u64) -> state -> result (state * unit)
+Axiom betree_utils_store_leaf_node
+  : u64 -> betree_List_t (u64 * u64) -> state -> result (state * unit)
 .
 
 (** [core::option::Option::{0}::unwrap]: forward function *)
-Axiom core_option_option_unwrap_fwd :
+Axiom core_option_Option_unwrap :
   forall(T : Type), option T -> state -> result (state * T)
 .
 
