tests/coq/misc/Constants.v
@@ -21,36 +21,35 @@ Definition x2_body : result u32 := Return 3%u32.
 Definition x2_c : u32 := x2_body%global.
 
 (** [constants::incr]: forward function *)
-Definition incr_fwd (n : u32) : result u32 :=
+Definition incr (n : u32) : result u32 :=
   u32_add n 1%u32.
 
 (** [constants::X3] *)
-Definition x3_body : result u32 := incr_fwd 32%u32.
+Definition x3_body : result u32 := incr 32%u32.
 Definition x3_c : u32 := x3_body%global.
 
 (** [constants::mk_pair0]: forward function *)
-Definition mk_pair0_fwd (x : u32) (y : u32) : result (u32 * u32) :=
-  Return (x, y)
-.
+Definition mk_pair0 (x : u32) (y : u32) : result (u32 * u32) :=
+  Return (x, y).
 
 (** [constants::Pair] *)
-Record Pair_t (T1 T2 : Type) := mkPair_t { Pair_x : T1; Pair_y : T2; }.
+Record Pair_t (T1 T2 : Type) := mkPair_t { pair_x : T1; pair_y : T2; }.
 
 Arguments mkPair_t {T1} {T2} _ _.
-Arguments Pair_x {T1} {T2}.
-Arguments Pair_y {T1} {T2}.
+Arguments pair_x {T1} {T2}.
+Arguments pair_y {T1} {T2}.
 
 (** [constants::mk_pair1]: forward function *)
-Definition mk_pair1_fwd (x : u32) (y : u32) : result (Pair_t u32 u32) :=
-  Return {| Pair_x := x; Pair_y := y |}
+Definition mk_pair1 (x : u32) (y : u32) : result (Pair_t u32 u32) :=
+  Return {| pair_x := x; pair_y := y |}
 .
 
 (** [constants::P0] *)
-Definition p0_body : result (u32 * u32) := mk_pair0_fwd 0%u32 1%u32.
+Definition p0_body : result (u32 * u32) := mk_pair0 0%u32 1%u32.
 Definition p0_c : (u32 * u32) := p0_body%global.
 
 (** [constants::P1] *)
-Definition p1_body : result (Pair_t u32 u32) := mk_pair1_fwd 0%u32 1%u32.
+Definition p1_body : result (Pair_t u32 u32) := mk_pair1 0%u32 1%u32.
 Definition p1_c : Pair_t u32 u32 := p1_body%global.
 
 (** [constants::P2] *)
@@ -59,31 +58,31 @@ Definition p2_c : (u32 * u32) := p2_body%global.
 
 (** [constants::P3] *)
 Definition p3_body : result (Pair_t u32 u32) :=
-  Return {| Pair_x := 0%u32; Pair_y := 1%u32 |}
+  Return {| pair_x := 0%u32; pair_y := 1%u32 |}
 .
 Definition p3_c : Pair_t u32 u32 := p3_body%global.
 
 (** [constants::Wrap] *)
-Record Wrap_t (T : Type) := mkWrap_t { Wrap_val : T; }.
+Record Wrap_t (T : Type) := mkWrap_t { wrap_value : T; }.
 
 Arguments mkWrap_t {T} _.
-Arguments Wrap_val {T}.
+Arguments wrap_value {T}.
 
 (** [constants::Wrap::{0}::new]: forward function *)
-Definition wrap_new_fwd (T : Type) (val : T) : result (Wrap_t T) :=
-  Return {| Wrap_val := val |}
+Definition wrap_new (T : Type) (value : T) : result (Wrap_t T) :=
+  Return {| wrap_value := value |}
 .
 
 (** [constants::Y] *)
-Definition y_body : result (Wrap_t i32) := wrap_new_fwd i32 2%i32.
+Definition y_body : result (Wrap_t i32) := wrap_new i32 2%i32.
 Definition y_c : Wrap_t i32 := y_body%global.
 
 (** [constants::unwrap_y]: forward function *)
-Definition unwrap_y_fwd : result i32 :=
-  Return y_c.(Wrap_val).
+Definition unwrap_y : result i32 :=
+  Return y_c.(wrap_value).
 
 (** [constants::YVAL] *)
-Definition yval_body : result i32 := unwrap_y_fwd.
+Definition yval_body : result i32 := unwrap_y.
 Definition yval_c : i32 := yval_body%global.
 
 (** [constants::get_z1::Z1] *)
@@ -91,11 +90,11 @@ Definition get_z1_z1_body : result i32 := Return 3%i32.
 Definition get_z1_z1_c : i32 := get_z1_z1_body%global.
 
 (** [constants::get_z1]: forward function *)
-Definition get_z1_fwd : result i32 :=
+Definition get_z1 : result i32 :=
   Return get_z1_z1_c.
 
 (** [constants::add]: forward function *)
-Definition add_fwd (a : i32) (b : i32) : result i32 :=
+Definition add (a : i32) (b : i32) : result i32 :=
   i32_add a b.
 
 (** [constants::Q1] *)
@@ -107,20 +106,19 @@ Definition q2_body : result i32 := Return q1_c.
 Definition q2_c : i32 := q2_body%global.
 
 (** [constants::Q3] *)
-Definition q3_body : result i32 := add_fwd q2_c 3%i32.
+Definition q3_body : result i32 := add q2_c 3%i32.
 Definition q3_c : i32 := q3_body%global.
 
 (** [constants::get_z2]: forward function *)
-Definition get_z2_fwd : result i32 :=
-  i <- get_z1_fwd; i0 <- add_fwd i q3_c; add_fwd q1_c i0
-.
+Definition get_z2 : result i32 :=
+  i <- get_z1; i0 <- add i q3_c; add q1_c i0.
 
 (** [constants::S1] *)
 Definition s1_body : result u32 := Return 6%u32.
 Definition s1_c : u32 := s1_body%global.
 
 (** [constants::S2] *)
-Definition s2_body : result u32 := incr_fwd s1_c.
+Definition s2_body : result u32 := incr s1_c.
 Definition s2_c : u32 := s2_body%global.
 
 (** [constants::S3] *)
@@ -128,7 +126,7 @@ Definition s3_body : result (Pair_t u32 u32) := Return p3_c.
 Definition s3_c : Pair_t u32 u32 := s3_body%global.
 
 (** [constants::S4] *)
-Definition s4_body : result (Pair_t u32 u32) := mk_pair1_fwd 7%u32 8%u32.
+Definition s4_body : result (Pair_t u32 u32) := mk_pair1 7%u32 8%u32.
 Definition s4_c : Pair_t u32 u32 := s4_body%global.
 
 End Constants .
