tests/coq/misc/External_Opaque.v
@@ -11,7 +11,7 @@ Import External_Types.
 Module External_Opaque.
 
 (** [core::mem::swap]: forward function *)
-Axiom core_mem_swap_fwd :
+Axiom core_mem_swap :
   forall(T : Type), T -> T -> state -> result (state * unit)
 .
 
@@ -26,12 +26,12 @@ Axiom core_mem_swap_back1 :
 .
 
 (** [core::num::nonzero::NonZeroU32::{14}::new]: forward function *)
-Axiom core_num_nonzero_non_zero_u32_new_fwd
-  : u32 -> state -> result (state * (option Core_num_nonzero_non_zero_u32_t))
+Axiom core_num_nonzero_NonZeroU32_new
+  : u32 -> state -> result (state * (option core_num_nonzero_NonZeroU32_t))
 .
 
 (** [core::option::Option::{0}::unwrap]: forward function *)
-Axiom core_option_option_unwrap_fwd :
+Axiom core_option_Option_unwrap :
   forall(T : Type), option T -> state -> result (state * T)
 .
 
